---
title: "P8104 Homework 3"
output: pdf_document
---

```{r setup, include=FALSE}
knitr::opts_chunk$set(echo = TRUE)
```

\begin{center}
\textbf{Nick Williams \\
ntw2117}
\end{center}

## Problem 1

(1) 

(2)

## Problem 2  

$$f_X(x) = 2xI\{0<x<1\}$$

(1) 
$$
\begin{aligned}
  Y = g(x) &= 4X - 3 \\
  \frac{d}{dx}g(x) &= 4 > 0 & \text{thus } g(x) \text{is an increasing function} \\
  g^{-1}(y) &= \frac{y + 3}{4} 
\end{aligned}
$$

$$
\begin{aligned}
  f_Y(y) &= f_X(g^{-1}(y))|\frac{d}{dy} g^{-1}(y)| \\
         &= f_X(\frac{y + 3}{4}) |\frac{1}{4}| & \frac{d}{dy}g^{-1}(y) = \frac{1}{4} \\
         &= 2\frac{y + 3}{4} (\frac{1}{4}) \\
         &= \frac{y + 3}{8} \text{ for } -3 < y < 1
\end{aligned}
$$

(2)
$$
\begin{aligned}
  Y = g(x) &= 3 - X^2 \\
  \frac{d}{dy}g(x) &= -2x < 0 & \text{ monotone }\forall \text{ } 0 < x < 1 \\
  g^{-1}(y) &= \sqrt{3 - y}
\end{aligned}
$$

$$
\begin{aligned}
  f_Y(y) &= f_X(g^{-1}(y))|\frac{d}{dy} g^{-1}(y)| \\
         &= f_x(\sqrt{3 - y}) \bigg|-\frac{1}{2 \sqrt{3 - y}}\bigg| & \frac{d}{dy}g^{-1}(y) = -\frac{1}{2\sqrt{3 - y}} \\
         &= f_x(\sqrt{3 - y}) \bigg(\frac{1}{2 \sqrt{3 - y}} \bigg) \\
         &= 2(\sqrt{3 - y}) \bigg(\frac{1}{2 \sqrt{3 - y}} \bigg) \\
         &= 1 \text{ for } 2 < y < 3
\end{aligned}
$$

## Problem 3

(1)  

(2)  
$$
\begin{aligned}
X \sim U(-1, 1) & & f_X(x) = \frac{1}{2} \text{ for } -1 \leq x \leq 1 \\
Y = g(x) = e^x & & g^{-1}(y) = log(x) \\
\end{aligned}
$$

Because $\frac{d}{dx} g(x) = e^x > 0$ $\forall x \in [-1, 1]$, $g(x)$ is an increasing function and monotone; therefore

$$
\begin{aligned}
  f_Y(y) &= f_X(g^{-1}(y)) \bigg|\frac{d}{dy} g^{-1}(y) \bigg| &   F_Y(y) &= F_X(g^{-1}(y)) \\
         &= \frac{1}{2} \bigg| \frac{1}{y} \bigg|              &          &= \frac{g^{-1}(y) + 1}{2} \\
         &= \frac{1}{2y}                                       &          &= \frac{\log(y) + 1}{2} \\
\end{aligned}
$$

\vspace{1cm}

$$
\begin{aligned}
X \sim U(-1, 1) & & f_X(x) = \frac{1}{2} \text{ for } -1 \leq x \leq 1 \\
Z = g(x) = -\log(X + 1) & & g^{-1}(z) = e^{-z} - 1 \\
\end{aligned}
$$

Because $\frac{d}{dx} g(z) = -\frac{1}{x + 1} < 0$ $\forall x \in [-1, 1]$, $g(x)$ is a decreasing function and monotone; therefore

$$
\begin{aligned}
  F_Z(z) &= 1 - F_X(g^{-1}(z))                      &   f_Z(z) &= f_X(g^{-1}(z)) \bigg|\frac{d}{dz} g^{-1}(z) \bigg| \\
         &= 1 - F_X(e^{-z} - 1)                     &          &= \frac{1}{2} \bigg| -e^{-z} \bigg| \\
         &= 1 - \frac{(e^{-z} - 1) + 1}{2}          &          &= \frac{e^{-z}}{2} \\
         &= - \frac{e^{-z}}{2}
\end{aligned}
$$






